changed to functional, proved structure

segmentTreeProof.dfy
@@ -68,248 +68,147 @@ module Monoid {
         constructor() {
         }
     }
-}
 
-/*predicate validTree<T(!new)>(tree: array<T>, monoid: Monoid.AbstractMonoid<T>) 
-reads tree
-requires monoid.validMonoid()
+}
+datatype SegmentTree<T> =
+    Leaf(m: int, value: T)
+    | Node(l: int, m: int, r: int, left: SegmentTree, right: SegmentTree, value: T)
+
+predicate validTree(st: SegmentTree)
+    decreases st
 {
-    forall i :: 0 < i < tree.Length / 2 ==> tree[i] == monoid.op(tree[2 * i], tree[2 * i + 1])
+    match st
+    {
+        case Leaf(_, _) =>
+            true
+
+        case Node(ll, mm, rr, left, right, _) =>
+            ll <= mm < rr
+            && validTree(left)
+            && validTree(right)
+            && (match left {
+                case Leaf(x, _) =>
+                    x == ll && x == mm
+                case Node(l2, m2, r2, _, _, _) =>
+                    l2 == ll && r2 == mm
+                })
+            && (match right {
+                case Leaf(x, _) =>
+                    x == rr && x == mm + 1
+                case Node(l2, m2, r2, _, _, _) =>
+                    l2 == mm + 1 && r2 == rr
+                })
+    }
 }
 
-method updateTree<T(!new)>(
-    index: int, 
-    n: int, 
-    elems: array<T>, 
-    monoid: Monoid.AbstractMonoid<T>, 
-    elem: T
-    ) returns  (res: array<T>)
-    requires elems.Length == 2 * n
-    requires forall i :: 0 <= i < n ==> elems[i] == monoid.op(elems[2 * i], elems[2 * i + 1]) 
+predicate validTreeValues<T(!new)>(tree: SegmentTree<T>, arr: array<T>, l: int, r: int, monoid: Monoid.AbstractMonoid<T>)
+    reads arr
+    requires 0 <= l <= r < arr.Length
+    requires validTree(tree)
+    requires boundaries(tree) == (l, r) 
+{
+    match tree {
+        case Leaf(l, val) => arr[l] == val
+        case Node(l, m, r, left, right, val) => 
+            validTreeValues(left, arr, l, m, monoid) && 
+            validTreeValues(right, arr, m + 1, r, monoid) &&
+            val == monoid.op(getValue(left), getValue(right))
+    }
+}
+
+function method boundaries(tree: SegmentTree): (int, int)
+{
+    match tree {
+        case Node(l, _, r, _, _, _) => (l, r)
+        case Leaf(x, _) => (x, x)
+    }
+}
+
+
+function method getValue<T>(tree: SegmentTree<T>): T
+{
+    match tree {
+        case Node(_, _, _, _, _, val) => val
+        case Leaf(_, val) => val
+    }
+}
+
+function method mergeTrees<T>(left: SegmentTree<T>, right: SegmentTree<T>, merge: (T, T) -> T): (res: SegmentTree<T>)
+    requires validTree(left)
+    requires validTree(right)
+    requires boundaries(left).1 + 1 == boundaries(right).0
+    ensures validTree(res)
+    ensures match res {
+        case Node(_, _, _, leftRes, rightRes, _) =>
+            left == left && right == right
+        case Leaf(_, _) => false
+    }
+    ensures getValue(res) == merge(getValue(left), getValue(right))
+{
+    Node(boundaries(left).0, boundaries(left).1, boundaries(right).1, left, right, merge(getValue(left), getValue(right)))
+}
+
+function method buildTree<T(!new)>(arr: array<T>, l: int, r: int, monoid: Monoid.AbstractMonoid<T>): (res: SegmentTree<T>)
+    reads arr
+    requires 0 <= l <= r < arr.Length
     requires monoid.validMonoid()
-    requires 0 <= index < n 
-    requires validTree(elems, monoid)
-    ensures validTree(res, monoid)
-    ensures res.Length == 2 * n
+    ensures boundaries(res) == (l, r)
+    ensures getValue(res) == straightQuery(arr, l, r, monoid)
+    ensures validTree(res)
+    ensures validTreeValues(res, arr, l, r, monoid)
+    decreases r - l
 {
-    var newTree := new T[2 * n](i => elem);
-    var i := 0;
-    while i < 2 * n 
-    invariant 0 <= i <= 2 * n
-    invariant forall j :: 0 <= j < i && j != index + n ==> newTree[j] == elems[j] 
-    {
-        if i != index + n {
-            newTree[i] := elems[i];
-        }
-        i := i + 1;
+    if l == r 
+    then Leaf(l, arr[l]) 
+    else (associativeQuery(arr, l, ((l + r) / 2), r, monoid); 
+    mergeTrees(
+        buildTree(arr, l, (l + r) / 2, monoid), 
+        buildTree(arr, (l + r) / 2 + 1, r, monoid), monoid.op))
+}
+
+function straightQuery<T(!new)>(elems: array<T>, l: int, r: int, monoid: Monoid.AbstractMonoid<T>): (res: T) 
+    reads elems
+    requires 0 <= l <= elems.Length && 0 <= r < elems.Length
+    requires monoid.hasIdentity()
+    ensures r == l ==> res == elems[l]
+    ensures r < l ==> res == monoid.identity()
+    decreases r - l
+{
+    if l > r then monoid.identity() else monoid.op(elems[l], straightQuery(elems, l + 1, r, monoid))
+}
+
+lemma associativeQuery<T(!new)>(elems: array<T>, l: int, m: int, r: int, monoid: Monoid.AbstractMonoid<T>) 
+    requires 0 <= l <= m <= r < elems.Length
+    requires monoid.validMonoid()
+    ensures straightQuery(elems, l, r, monoid) == monoid.op(straightQuery(elems, l, m, monoid), straightQuery(elems, m + 1, r, monoid))
+    decreases r - l
+{
+    if (r == m) {
+        assert straightQuery(elems, l, r, monoid) == monoid.op(straightQuery(elems, l, m, monoid), straightQuery(elems, m + 1, r, monoid));
+        return;
     }
-    var pnt := index + n;
-    pnt := pnt / 2;
-    while pnt > 0
-    invariant 0 <= pnt < n
-    invariant forall vert :: (0 < vert < pnt) && (vert / 2 != pnt) ==> newTree[vert] == monoid.op(newTree[2 * vert], newTree[2 * vert + 1])
-    {
-        pnt := pnt / 2;
-    }
-    return newTree;
-}*/
-
-predicate isPowerTwo(s: bv32)
-{
-    s > 0 && (s & (s - 1) == 0)
+    assert straightQuery(elems, l, r, monoid) == monoid.op(straightQuery(elems, l, m, monoid), straightQuery(elems, m + 1, r, monoid));
 }
 
-predicate allSplit(splitSeq: seq<(int, int)>, start: int, end: int)
+class SegmentTreeWrapper<T(!new)>
 {
-    |splitSeq| == 0 || (splitSeq[0].0 == start && splitSeq[|splitSeq| - 1].1 == end &&
-    forall i :: 0 < i < |splitSeq| ==> splitSeq[i - 1].1 + 1 == splitSeq[i].0)
-}
-
-predicate powTwoSeq(splitSeq: seq<(int, int)>, twoPower: int) 
-    requires twoPower >= 1
-    //requires isPowerTwo(twoPower)
-{
-    |splitSeq| == 0 || (forall i :: 0 <= i < |splitSeq| ==> splitSeq[i] == (twoPower * i, twoPower * (i + 1) - 1))
-}
-
-
-lemma powTwoDiv(x: bv32, y: bv32) 
-    requires x >= y >= 1
-    requires isPowerTwo(x)
-    requires isPowerTwo(y)
-    ensures isPowerTwo(x / y)
-{
-    assert isPowerTwo(x / y);
-}
-
-/*method createBoundaries(n: int) returns (res: array<(int, int)>)
-    requires n > 1 
-    requires isPowerTwo(n)
-    ensures res.Length == n
-    //ensures forall twoPower: nat :: isPowerTwo(twoPower) && 1 <= twoPower <= n / 2 ==> allSplit(res[twoPower..2 * twoPower], 0, n / 2 - 1)
-    //ensures forall i :: 1 <= i < n / 2 ==> res[i] == (res[2 * i].0, res[2 * i + 1].1)
-    decreases n
-{
-    if (n == 2) {
-        var arr := new (int, int)[2];
-        arr[1] := (0, n / 2 - 1);
-        //assert forall twoPower: nat :: isPowerTwo(twoPower) && 1 <= twoPower <= n / 2 ==> allSplit(arr[twoPower .. 2 * twoPower], 0, n / 2 - 1);
-        return arr;
-    } 
-    var arr := new (int, int)[n];
-    var twoPower := n / 2;
-    var compTwoPower := 1;
-    var index := twoPower;
-    while index < twoPower * 2
-        invariant twoPower <= index <= 2 * twoPower
-        invariant forall grtTwoPower: nat :: isPowerTwo(grtTwoPower) && 2 * twoPower <= grtTwoPower <= n / 2 ==> 
-            powTwoSeq(arr[grtTwoPower..2 * grtTwoPower], n / 2 / grtTwoPower)
-        //invariant forall j :: twoPower <= j <= index ==> allSplit(arr[twoPower..j], 0, (j - twoPower) * compTwoPower - 1)
-        //invariant forall grtTwoPower: nat :: isPowerTwo(grtTwoPower) && 2 * twoPower <= grtTwoPower <= n / 2 ==> 
-        //    allSplit(arr[grtTwoPower..2 * grtTwoPower], 0, n / 2 - 1)    
-    {
-        arr[index] := ((index - twoPower) * compTwoPower, (index - twoPower) * compTwoPower + compTwoPower - 1);
-        index := index + 1;
-    }
-    twoPower := twoPower / 2;
-    compTwoPower := compTwoPower * 2;
-    
-    while twoPower > 1
-        invariant 1 <= twoPower <= n
-        invariant isPowerTwo(twoPower)
-        invariant isPowerTwo(compTwoPower)
-        invariant compTwoPower * twoPower == n / 2 
-        invariant forall grtTwoPower: nat :: isPowerTwo(grtTwoPower) && 2 * twoPower <= grtTwoPower <= n / 2 ==> 
-            powTwoSeq(arr[grtTwoPower..2 * grtTwoPower], n / 2 / grtTwoPower)
-        //invariant forall grtTwoPower: nat :: isPowerTwo(grtTwoPower) && 2 * twoPower <= grtTwoPower <= n / 2 ==> 
-        //    allSplit(arr[grtTwoPower..2 * grtTwoPower], 0, n / 2 - 1)
-    {
-        var i := twoPower;
-        while i < twoPower * 2
-            invariant twoPower <= i <= 2 * twoPower
-            invariant forall j :: twoPower <= j < i ==> arr[j] == ((j - twoPower) * compTwoPower, (j - twoPower) * compTwoPower + compTwoPower - 1)
-            invariant forall j :: twoPower <= j <= i ==> allSplit(arr[twoPower..j], 0, (j - twoPower) * compTwoPower - 1)
-            //invariant forall grtTwoPower: nat :: isPowerTwo(grtTwoPower) && 2 * twoPower <= grtTwoPower <= n / 2 ==> 
-            //    allSplit(arr[grtTwoPower..2 * grtTwoPower], 0, n / 2 - 1)    
-        {
-            //assert allSplit(arr[twoPower..i], 0, (i - twoPower) * compTwoPower - 1);
-            arr[i] := ((i - twoPower) * compTwoPower, (i - twoPower) * compTwoPower + compTwoPower - 1);
-            i := i + 1;
-        }
-        //assert allSplit(arr[twoPower..twoPower * 2], 0, n / 2 - 1);
-        //powerTwoIneq(twoPower); 
-        //assert forall grtTwoPower: nat :: isPowerTwo(grtTwoPower) && 2 * twoPower <= grtTwoPower <= n / 2 ==> 
-        //    allSplit(arr[grtTwoPower..2 * grtTwoPower], 0, n / 2 - 1);
-        twoPower := twoPower / 2;
-        compTwoPower := compTwoPower * 2;
-        //assert forall grtTwoPower: nat :: isPowerTwo(grtTwoPower) && 2 * twoPower <= grtTwoPower <= n / 2 ==> 
-        //    grtTwoPower == 2 * twoPower || grtTwoPower >= twoPower * 4;
-        //assert forall grtTwoPower: nat :: isPowerTwo(grtTwoPower) && 4 * twoPower <= grtTwoPower <= n / 2 ==> 
-        //    allSplit(arr[grtTwoPower..2 * grtTwoPower], 0, n / 2 - 1);
-    }
-    //assert forall grtTwoPower: nat :: isPowerTwo(grtTwoPower) && 2 <= grtTwoPower <= n / 2 ==> 
-    //        allSplit(arr[grtTwoPower..2 * grtTwoPower], 0, n / 2 - 1);
-    arr[1] := (0, n / 2 - 1);
-    return arr;
-}
-*/
-
-class SegmentTree<T(!new, ==)> {
-    var monoid: Monoid.AbstractMonoid<T>
     var elems: array<T>
-    var boundaries: array<(int, int)>
-    var n: nat
-    predicate validSize() 
-        reads this
-        requires n <= 10_000
-    {
-        2 * n == elems.Length && isPowerTwo(n as bv32)
-    }
-    constructor(m: Monoid.AbstractMonoid<T>, size: int) 
-        requires size >= 1
-        requires size <= 1_000
+    var tree: SegmentTree<T>
+    var monoid: Monoid.AbstractMonoid<T>
+
+    constructor(arr: array<T>, m: Monoid.AbstractMonoid<T>) 
         requires m.validMonoid()
-        ensures n >= size
-        ensures size * 2 >= n
-        ensures validSize()
-        ensures valid()
+        requires arr.Length > 0
         ensures monoid.validMonoid()
+        ensures elems.Length == arr.Length
+        ensures validTree(tree)
+        ensures boundaries(tree) == (0, elems.Length - 1)
+        ensures validTreeValues(tree, elems, 0, elems.Length - 1, monoid)
     {
-        monoid := m;
-        var hf: bv32 := 1 as bv32;
-        while (hf as int < size)
-            invariant 1 <= hf as int <= size * 2
-            invariant isPowerTwo(hf)
-        {
-            hf := hf >> 1;
-        }
-        n := hf as int;
-        assert hf as int <= 2 * size;
-        elems := new T[2 * hf as int](i => m.identity());
-    }
-    predicate valid() 
-        reads this
-        reads elems
-        requires n < 10_000
-        requires validSize()
-    {
-        forall i: int :: 0 < i < n ==> elems[i] == monoid.op(elems[2 * i], elems[2 * i + 1])
-    }
-
-    /*method setBoundaries()
-        modifies this
-        requires isPowerTwo(n) && n >= 1
-        ensures boundaries.Length == 2 * n
-        ensures forall lvl: nat :: isPowerTwo(lvl) && 1 <= lvl <= n ==> allSplit(boundaries[lvl..lvl * 2], 0, n - 1)
-    {   
-        boundaries := createBoundaries(2 * n);
-    }*/
-    
-    /*method changeElement(index: int, elem: T)
-        modifies elems
-        requires 0 <= index < n
-        requires validSize()
-        requires valid()
-        ensures valid()
-        ensures elems[index + n] == elem
-    {
-        var pnt := index + n;
-        elems[pnt] := elem;
-        while pnt > 1
-            invariant forall i: int :: 0 < i < n && 2 * i != pnt && 2 * i + 1 != pnt ==> elems[i] == monoid.op(elems[2 * i], elems[2 * i + 1])
-            invariant elems[index + n] == elem
-            invariant pnt / 2 < n
-        {
-            pnt := pnt / 2;
-            elems[pnt] := monoid.op(elems[pnt * 2], elems[pnt * 2 + 1]);
-        }
-    }*/
-
-    function straightQuery(l: int, r: int): (res: T) 
-        reads this
-        reads elems
-        requires 0 <= l <= n && 0 <= r < n
-        requires validSize()
-        requires monoid.hasIdentity()
-        ensures r == l ==> res == elems[l + n]
-        ensures r < l ==> res == monoid.identity()
-        decreases n - l
-    {
-        if l > r then monoid.identity() else monoid.op(elems[l + n], straightQuery(l + 1, r))
-    }
-
-    lemma associativeQuery(l: int, r: int, m: int) 
-        requires 0 <= l <= m <= r < n
-        requires validSize()
-        requires monoid.validMonoid()
-        ensures straightQuery(l, r) == monoid.op(straightQuery(l, m), straightQuery(m + 1, r))
-        decreases r - l
-    {
-        if (r == m) {
-            assert straightQuery(l, r) == monoid.op(straightQuery(l, m), straightQuery(m + 1, r));
-            return;
-        }
-        assert straightQuery(l, r) == monoid.op(straightQuery(l, m), straightQuery(m + 1, r));
+        elems := arr;
+        var mon := m;
+        tree := buildTree(arr, 0, arr.Length - 1, mon);
+        monoid := mon;
     }
 }
 
@@ -318,11 +217,6 @@ method Main() {
     var minMonoidInstance := new Monoid.MinMonoid();
     var minMonoidSt := new Monoid.MinMonoid();
     assert minMonoidSt.validMonoid();
-    var segmentTreeInstance := new SegmentTree<Monoid.BoundedInt>(minMonoidSt, 6);
-    print segmentTreeInstance.elems[0], "\n";
-    assert segmentTreeInstance.validSize();
-    //segmentTreeInstance.changeElement(0, 8);
-    //print segmentTreeInstance.straightQuery(0, 1);
     print addMonoidInstance.op(3, 13), " ";
     print addMonoidInstance.identity(), " ";
     print minMonoidInstance.op(3, 13), " ";
